Add files via upload

proiect.v
@@ -1,20 +1,18 @@
 Require Import String.
-Inductive identif := a | b | c | d | e | f | g | h | i.
+Inductive identif := a | b | c | d | e | f | g | h | i | n | s.
 
 Inductive Value :=
 | undefined : Value
 | Number : nat -> Value
 | Boolean : bool -> Value.
 
-Definition Env : identif -> Value.
-
 Inductive Exp :=
-| evar : Value -> Exp
+| evar : identif -> Exp
 | estring : string -> Exp
 | enum : nat -> Exp
 | plus : Exp -> Exp -> Exp
 | times : Exp -> Exp -> Exp
-| div : Exp -> Exp -> Exp
+| div : Exp -> Exp -> Exp (**)
 | minus : Exp -> Exp -> Exp
 | true : Exp
 | false : Exp
@@ -43,33 +41,210 @@ Notation "A &&' B" := (and A B) (at level 60).
 Notation "A ||' B" := (or A B) (at level 61).
 Notation "A == B" := (beqto A B) (at level 62).
 Notation "A != B" := (notbeqto A B) (at level 62).
-Notation "A === B" := (eqValeqType A B) (at level 62).
-Notation "A !== B" := (noteqValeqType A B) (at level 62).
+(*Notation "A === B" := (eqValeqType A B) (at level 62).
+Notation "A !== B" := (noteqValeqType A B) (at level 62).*)
 Notation "' A '" := (estring A) (at level 62).
 
 Coercion enum : nat >-> Exp.
+Coercion evar : identif >-> Exp.
 
 Compute (true +' 1).
 Compute (true +' true).
 Compute (true == 1).
 Compute (' "str" ').
+Compute (1 <' 2).
 
 Inductive Statement :=
 | declaration : identif -> Statement
-| assign : identif -> Value -> Statement
+| assign : identif -> Exp -> Statement
 | sequence : Statement -> Statement -> Statement
 | ifElse : Exp -> Statement -> Statement -> Statement
 | ifThen : Exp -> Statement -> Statement
-| while : Exp -> Statement -> Statement
-| For : Statement -> Exp -> Exp -> Statement -> Statement.
+| While : Exp -> Statement -> Statement
+| For : Statement -> Exp -> Statement -> Statement -> Statement.
 
-Notation "'var' A" := (declaration A) (at level 100).
 Notation "'Let' A" := (declaration A) (at level 100).
-Notation "'const' A" := (declaration A) (at level 100).
 Notation "A =' B" := (assign A B) (at level 101).
-Notation "A ; B" := (sequence A B) (at level 101).
-Notation "'If' A { B } 'Else' { C }" := (ifElse A B C) (at level 102).
-Notation "'If' A { B }" := (ifThen A B) (at level 90).
+Notation "A ; B" := (sequence A B) (at level 102).
+Notation "'If' ( A ) { B } 'Else' { C }" := (ifElse A B C) (at level 102).
+Notation "'If' A 'Then' B " := (ifThen A B) (at level 102).
+Notation "'while' ( A ) { B }" := (While A B) (at level 102).
+Notation "'For' ( A ;; B ;; C ) { D }" := (For A B C D) (at level 102).
+
+
+
+Scheme Equality for identif. 
+ 
+Definition Env := identif -> nat.
+
+Definition envA : Env :=
+  fun var =>
+  if (identif_eq_dec var a)
+          then 1
+  else if (identif_eq_dec var b)
+          then 10
+  else if (identif_eq_dec var c)
+          then 15
+  else if (identif_eq_dec var d)
+          then 20
+  else if (identif_eq_dec var e)
+          then 4
+  else 0.
+
+Definition update (env : Env) (z : identif) (value : nat) : Env :=
+  fun var =>
+    if(identif_eq_dec var z)
+      then value
+    else (env var).
+
+Notation "S [ V /' X ]" := (update S X V) (at level 0).
+
+Reserved Notation "A =[ State ]=> N" (at level 60).
+Inductive exp_eval : Exp -> Env -> nat -> Prop :=
+| const : forall n sigma, enum n =[ sigma ]=> n  
+| var : forall v sigma, evar v =[ sigma ]=> (sigma v)
+| add : forall a1 a2 i1 i2 sigma result,
+  a1 =[ sigma ]=> i1 ->
+  a2 =[ sigma ]=> i2 ->
+  result = i1 + i2 ->
+  a1 +' a2 =[ sigma ]=> result
+| timesEval : forall a1 a2 i1 i2 sigma result,
+  a1 =[ sigma ]=> i1 ->
+  a2 =[ sigma ]=> i2 ->
+  result = i1 * i2 ->
+  a1 *' a2 =[ sigma ]=> result
+| div_not_0 : forall a1 a2 i1 i2 sigma result,
+  a1 =[ sigma ]=> i1 ->
+  a2 =[ sigma ]=> i2 ->
+  result = Nat.div i1 i2 ->
+  a1 /' a2 =[ sigma ]=> result
+| div_0 : forall a1 a2 i1 sigma,
+  a1 =[ sigma ]=> i1 ->
+  a2 =[ sigma ]=> 0 ->
+  a1 /' a2 =[ sigma ]=> 0
+| minusEval : forall a1 a2 i1 i2 sigma result,
+  a1 =[ sigma ]=> i1 ->
+  a2 =[ sigma ]=> i2 ->
+  result = i1 - i2 ->
+  a1 -' a2 =[ sigma ]=> result
+| trueEval : forall state, true =[ state ]=> 1
+| falseEval : forall state, false =[ state ]=> 0
+| lessthanEval : forall a1 i1 a2 i2 state comp,
+  a1 =[ state ]=> i1 ->
+  a2 =[ state ]=> i2 ->
+  comp = Nat.ltb i1 i2 ->
+  a1 <' a2 =[ state ]=> if(comp) then 1 else 0
+| lesseqthanEval : forall a1 i1 a2 i2 state,
+  a1 =[ state ]=> i1 ->
+  a2 =[ state ]=> i2 ->
+  a1 <=' a2 =[ state ]=> if(Nat.leb i1 i2) then 1 else 0
+| greaterthanEval : forall a1 i1 a2 i2 state,
+  a1 =[ state ]=> i1 ->
+  a2 =[ state ]=> i2 ->
+  a1 >' a2 =[ state ]=> if(Nat.ltb i2 i1) then 1 else 0
+| greatereqthan : forall a1 i1 a2 i2 state,
+  a1 =[ state ]=> i1 ->
+  a2 =[ state ]=> i2 ->
+  a1 >=' a2 =[ state ]=> if (Nat.leb i2 i1) then 1 else 0
+| eqtoEval : forall a1 a2 i1 i2 state comp,
+  a1 =[ state ]=> i1 ->
+  a2 =[ state ]=> i2 ->
+  comp = Nat.eqb i1 i2 ->
+  (beqto a1 a2) =[ state ]=> if (comp) then 1 else 0
+| neqtoEval : forall a1 a2 i1 i2 state comp, 
+  a1 =[ state ]=> i1 -> 
+  a2 =[ state ]=> i2 ->
+  comp = Nat.eqb i1 i2 ->
+  (notbeqto a1 a2) =[ state ]=> if (comp) then 0 else 1
+where "a =[ s ]=> n" := (exp_eval a s n).
+
+Require Import Omega.
+
+Example e1 : 3 +' a *' 2 =[ envA ]=> 5.
+Proof.
+  eapply add.
+  eapply const.
+  eapply timesEval.
+  eapply var.
+  eapply const.
+  eauto.
+  eauto.
+Qed.
+
+Example e2 : 1 +' true =[ envA ]=> 2.
+Proof.
+  eapply add.
+  eapply const.
+  eapply trueEval.
+  omega.
+Qed.
+
+Reserved Notation " S ={ state }=> state'" (at level 60).
+Inductive Stmt_eval : Statement -> Env -> Env -> Prop :=
+| assign_eval : forall a i x state1 state2,
+    a =[ state1 ]=> i ->
+    state2 = (update state1 x i) ->
+    (x =' a) ={ state1 }=> state2
+| seq_eval : forall s1 s2 state state1 state2,
+    s1 ={ state }=> state1 -> 
+    s2 ={ state1 }=> state2 ->
+    (s1 ; s2) ={ state }=> state2 
+| if_true_eval : forall cond s1 s2 state state',
+    cond =[ state ]=> 1 ->
+    s1 ={ state }=> state'->
+    ifElse cond s1 s2 ={ state }=> state'
+| if_false_eval : forall cond s1 s2 state state',
+    cond =[state]=> 0 ->
+    s2 ={ state }=> state'->
+    ifElse cond s1 s2 ={ state }=> state'  
+| while_true : forall cond s1 state state',
+    cond =[ state ]=> 1 ->
+    s1 ={ state }=> state' ->
+    While cond s1 ={ state }=> state'
+| while_false : forall cond s1 state,
+    cond =[ state ]=> 0 ->
+    While cond s1 ={ state }=> state
+where "s ={ state }=> state'" := (Stmt_eval s state state').
+
+Definition program :=
+  a =' 2 +' true ;
+  If ( a == 2 ) { a =' 4 } Else { a =' 5 } ;
+  c =' 4;
+  
+  while ( a <' c ) { a =' a +' 1 }  
+.
+
+Definition stateFirst := fun (x : identif) => 0.
+
+Example evalProgram : exists state, program ={ stateFirst }=> state /\ state a = 4.
+Proof.
+  eexists.
+  split.
+  unfold program.
+  eapply seq_eval.
+  eapply assign_eval.
+  eapply add. 
+  eapply const.
+  eauto.
+  eapply trueEval.
+  eauto.
+  eauto.
+  eapply seq_eval.
+  eapply seq_eval.  
+  eapply if_false_eval.
+  simpl.
+
+Abort.
+  
+  
+
+
+
+
+  
+
+
+
 
 
 
